Protocols/RBABC/Liveness_tla.v
@@ -1,0 +1,81 @@
+From Coq Require Import List Bool Lia PeanoNat ListSet Permutation RelationClasses ClassicalChoice.
+From Coq Require ssrbool ssreflect.
+Import (coercions) ssrbool.
+Import ssreflect.SsrSyntax.
+From ABCProtocol.Protocols.RBABC Require Export Network.
+From ABCProtocol.Protocols.ABC Require Import Liveness_tla.
+From ABCProtocol.Protocols.RB Require Import Liveness_tla.
+
+Module RBACLiveness2 (A : NetAddr) (R : Round) (ARP : AddrRoundPair A R) (Sn : Signable) (V : SignableValue Sn) (VBFT : ValueBFT A R V) 
+  (BTh : ClassicByzThreshold A) (BSett : RestrictedByzSetting A BTh)
+  (P : PKI A Sn) (TSS0 : ThresholdSignatureSchemePrim A Sn with Definition thres := BTh.t0) (* ! *)
+  (TSS : ThresholdSignatureScheme A Sn with Module TSSPrim := TSS0).
+
+Import A R ARP V VBFT BTh BSett P TSS0 TSS.
+Import ssrbool. (* anyway *)
+
+Module RBLiveTLA := RBLiveness2 A R V VBFT BTh BSett.
+Module ACLiveTLA := ACLiveness2 A Sn V BTh BSett P TSS0 TSS.
+
+Import RBLiveTLA.RBLive.RBS.RBInv ACLiveTLA.ACLive.ACS.ACInv.
+
+Module Export RBACN := RBACNetwork A R ARP Sn V VBFT BTh BSett P TSS0 TSS RBN ACN.
+
+Include LivenessTLA A M BTh BSett Pk PSOp RBACP Ns RBACAdv RBACN.
+
+Definition exec_proj1 (e : exec World) : exec RBN.Ns.World := fun n => world_proj1 (e n).
+
+Definition exec_proj2 (e : exec World) : exec ACN.Ns.World := fun n => world_proj2 (e n).
+(*
+Definition next_proj1 (w1 w1' : RBN.Ns.World) : Prop :=
+  forall q w w', system_step q w w' -> RBN.system_step (ssd_proj1 q) w1 w1'.
+*)
+(*
+Fact next_proj1_sound w1 w1' : next_proj1 w1 w1' -> RBLiveTLA.next w1 w1'.
+Proof. intros H. hnf in H |- *. 
+*)
+(* TODO it seems inevitable to use some kind of choice axiom to prove the existence below?
+    sounds like reasonable, since we are reasoning about infinity *)
+Fact exec_proj1_sound (e : exec World) (H : e ⊨ □ ⟨ next ⟩) :
+  ∃ (e' : exec RBN.Ns.World), 
+    RBLiveTLA.exec_rel e' (exec_proj1 e) ∧
+    (e' ⊨ □ ⟨ RBLiveTLA.next ⟩).
+    (* (e' ⊨ □ ⟨ next_proj1 ⟩). *)
+Proof.
+  autounfold with tla in H. setoid_rewrite drop_n in H. simpl in H.
+  pose proof (choice _ H) as (f & Hf). clear H.   (* !!!!!!!! *)
+  pose (e' := RBN.final_world_n (fun n => (ssd_proj1 (f n))) (world_proj1 (e 0))).
+  exists e'. apply and_wlog_r.
+  - hnf. intros n. unfold exec_proj1. subst e'.
+    induction n as [ | n IH ]; try reflexivity.
+    rewrite RBN.final_world_n_add_1.
+    pose proof (ssd_proj1_sound _ _ _ (Hf n)) as (_ & H).
+    rewrite -H. now apply RBN.next_world_preserves_World_rel.
+  - intros Hrel.
+    split_and?; autounfold with tla.
+    + intros k. exists (ssd_proj1 (f k)). rewrite !drop_n /=. 
+      pose proof (ssd_proj1_sound _ _ _ (Hf k)) as (Ha & Hb).
+      subst e'. rewrite RBN.final_world_n_add_1. eapply RBN.step_mirrors_World_rel.
+      1: symmetry; apply Hrel. 1: apply Ha. 1: intros; auto. (* nice *)
+      specialize (Hrel (S k)). rewrite RBN.final_world_n_add_1 in Hrel. rewrite Hb Hrel. reflexivity.
+    (* + intros k. hnf. intros q w w' Hstep. rewrite !drop_n /=.
+      pose proof (ssd_proj1_sound _ _ _ Hstep) as (Ha & Hb).
+      subst e'. rewrite RBN.final_world_n_add_1. eapply RBN.step_mirrors_World_rel. *)
+Qed.
+
+Fact exec_proj1_sound_fairness (e : exec World) (H : e ⊨ □ ⟨ next ⟩)
+  (e' : exec RBN.Ns.World) (Hrel : RBLiveTLA.exec_rel e' (exec_proj1 e))
+  (H' : e' ⊨ □ ⟨ RBLiveTLA.next ⟩) :
+  (e ⊨ fairness) → (e' ⊨ RBLiveTLA.fairness).
+Proof.
+  (* change view *)
+  intros Hfair%fairness_adequate; auto. apply RBLiveTLA.fairness_adequate; auto.
+  hnf in Hfair |- *. intros [ src dst msg ? ] (Hs & Hd). simpl in *. intros -> n Hin.
+  specialize (Hfair (mkP src dst (inl msg) false) (conj Hs Hd) eq_refl n).
+  apply (proj2 (Hrel n)) in Hin. unfold exec_proj1, world_proj1 in Hin. simpl in Hin.
+  apply option_map_list_In in Hin. destruct Hin as ([ ? ? [] ? ] & Hin & Hpj); try discriminate.
+  cbn in Hpj. revert Hpj. intros [= -> -> -> ->]. specialize (Hfair Hin).
+  destruct Hfair as (k & Hstep). 
+Abort.
+
+End RBACLiveness2.
