Protocols/RBABC/Network.v
@@ -183,21 +183,24 @@ Local Hint Rewrite -> RBN.PC.In_consume ACN.PC.In_consume In_consume option_map_
 
 (* the definitions should be sound *)
 
-Fact ssd_proj1_sound q w w' (Hstep : system_step q w w') :
-  exists ww, RBN.system_step (ssd_proj1 q) (world_proj1 w) ww /\
+Fact ssd_proj1_sound q w :
+  let: ww := RBN.next_world (ssd_proj1 q) (world_proj1 w) in
+  forall w' (Hstep : system_step q w w'),
+    RBN.system_step (ssd_proj1 q) (world_proj1 w) ww /\
     RBN.Ns.World_rel ww (world_proj1 w').
 Proof.
+  intros w' Hstep.
   inversion_step' Hstep; clear Hstep; simpl.
   all: unfold world_proj1; simpl_world.
-  - eexists. split; [ constructor; reflexivity | ]. reflexivity.
+  - split; [ constructor | ]; reflexivity.
   - destruct msg as [ mRB | mAC ]; simpl.
-    + eexists. split; [ eapply RBN.DeliverStep; try reflexivity; simpl; auto | ].
+    + unfold stmap_proj1.
+      rewrite -> (surjective_pairing (RBN.RBP.procMsgWithCheck _ _ _)).
+      split; [ eapply RBN.DeliverStep; try reflexivity; simpl; auto | ].
       * apply option_map_list_In. eexists. split. apply Hpin. reflexivity.
-      * unfold stmap_proj1 at 1.
-        pose proof (procMsgWithCheck_proj1 _ _ _ _ _ Ef) as (E1 & E2).
-        rewrite -> (surjective_pairing (RBN.RBP.procMsgWithCheck _ _ _)), <- E1, <- E2.
-        reflexivity.
-      * hnf; simpl. split; [ intros ?; unfold stmap_proj1, upd, RBN.Ns.upd; now destruct_eqdec as_ -> | ].
+      * rewrite -> (surjective_pairing (RBN.RBP.procMsgWithCheck _ _ _)). reflexivity.
+      * pose proof (procMsgWithCheck_proj1 _ _ _ _ _ Ef) as (E1 & E2). rewrite <- E1, <- E2.
+        hnf; simpl. split; [ intros ?; unfold upd, RBN.Ns.upd; now destruct_eqdec as_ -> | ].
         hnf. intros p. unfold pkts_filter_proj1. autorewrite with psent.
         (* TODO cumbersome ... *)
         split.
@@ -214,7 +217,7 @@ Proof.
           ++right. right. split; eauto. intros <-. apply Hneq. 
             destruct a as [ ? ? [] ? ]; cbn in Hpj |- *; try discriminate.
             congruence.
-    + eexists. split; [ eapply RBN.IdleStep; try reflexivity; simpl; auto | ].
+    + split; [ eapply RBN.IdleStep; try reflexivity; simpl; auto | ].
       rewrite -> (surjective_pairing (ACN.ACP.procMsgWithCheck _ _ _)) in Ef.
       revert Ef. intros [= <- <-]. 
       hnf; simpl. split; [ intros ?; unfold stmap_proj1, upd, RBN.Ns.upd; now destruct_eqdec as_ -> | ].
@@ -225,12 +228,12 @@ Proof.
         autorewrite with psent. right. right. split; auto. intros <-. discriminate.
       * intros (a & Hin & Hpj). exists a. split; auto.
         autorewrite with psent in Hin. destruct Hin as [ (a' & <- & Hin')%in_map_iff | [ <- | (? & ?) ] ]; auto; try discriminate.
-  - eexists. split; [ eapply RBN.InternStep; try reflexivity; simpl; auto | ].
-    1: rewrite -> (surjective_pairing (RBN.RBP.procInt _ _)); reflexivity.
-    unfold stmap_proj1 at 1. unfold procInt in E.
-    rewrite -> (surjective_pairing (RBN.RBP.procInt _ _)) in E.
+  - unfold stmap_proj1. unfold procInt in E.
+    rewrite -> (surjective_pairing (RBN.RBP.procInt _ _)) in E |- *.
     revert E. intros [= <- <-].
-    hnf; simpl. split; [ intros ?; unfold stmap_proj1, upd, RBN.Ns.upd; now destruct_eqdec as_ -> | ].
+    split; [ eapply RBN.InternStep; try reflexivity; simpl; auto | ].
+    1: rewrite -> (surjective_pairing (RBN.RBP.procInt _ _)); reflexivity.
+    hnf; simpl. split; [ intros ?; unfold upd, RBN.Ns.upd; now destruct_eqdec as_ -> | ].
     hnf. intros p. unfold pkts_filter_proj1. autorewrite with psent.
     (* TODO cumbersome ... *)
     split.
@@ -240,7 +243,7 @@ Proof.
     + intros (a & Hin & Hpj). autorewrite with psent in Hin. destruct Hin as [ (p' & <- & Hin')%in_map_iff | Hin ]; eauto.
       apply pkt_proj1_refl_must in Hpj. subst. tauto.
   - destruct m as [ mRB | mAC ]; simpl.
-    + eexists. split; [ eapply RBN.ByzStep; try reflexivity; simpl; auto | ].
+    + split; [ eapply RBN.ByzStep; try reflexivity; simpl; auto | ].
       simpl. hnf; simpl. split; auto.
       hnf. intros p. unfold pkts_filter_proj1. autorewrite with psent.
       (* TODO cumbersome ... *)
@@ -250,7 +253,7 @@ Proof.
         --exists a. autorewrite with psent. tauto.
       * intros (a & Hin & Hpj). autorewrite with psent in Hin. destruct Hin as [ <- | Hin ]; eauto.
         cbn in Hpj. injection Hpj as <-. now left.
-    + eexists. split; [ eapply RBN.IdleStep; try reflexivity; simpl; auto | ].
+    + split; [ eapply RBN.IdleStep; try reflexivity; simpl; auto | ].
       hnf; simpl. split; auto.
       hnf. intros p. unfold pkts_filter_proj1. autorewrite with psent.
       setoid_rewrite In_sendout1. firstorder. subst. discriminate.
